theories/Data/FiniteMap.v
@@ -1,0 +1,27 @@
+Require Import PnV.Prelude.Prelude.
+
+#[local] Infix "=~=" := is_similar_to : type_scope.
+#[local] Infix "∈" := L.In.
+
+#[universes(polymorphic=yes), projections(primitive)]
+Record alist@{u v} {K : Type@{u}} {V : Type@{v}} : Type@{max(u, v)} :=
+  mk_alist { kvlist : list (K * V) } as al.
+
+#[global] Arguments alist : clear implicits.
+
+#[universes(polymorphic=yes)]
+Definition Similarity_alist_finite_partial_map {KEY : Type} {VAL : Type} {VAL' : Type} (VAL_sim : Similarity VAL VAL') : Similarity (alist KEY VAL) (KEY -> option VAL') :=
+  fun al : alist KEY VAL => fun m' : KEY -> option VAL' => forall key, ⟪ SUBMAP1 : forall val, (key, val) ∈ al.(kvlist) -> (exists val', val =~= val' /\ m' key = Some val') ⟫ /\ ⟪ SUBMAP2 : forall val', m' key = Some val' -> (exists val, val =~= val' /\ (key, val) ∈ al.(kvlist)) ⟫.
+
+#[global, universes(polymorphic=yes)]
+Instance alist_corresponds_to_finite_partial_map {KEY : Type} {VAL : Type} : Similarity (alist KEY VAL) (KEY -> option VAL) :=
+  Similarity_alist_finite_partial_map eq.
+
+#[universes(polymorphic=yes)]
+Theorem alist_corresponds_to_finite_partial_map_iff (KEY : Type) (VAL : Type) (al : alist KEY VAL) (m : KEY -> option VAL)
+  : al =~= m <-> (forall k, forall v, (k, v) ∈ al.(kvlist) <-> m k = Some v).
+Proof.
+  done!.
+Qed.
+
+#[global] Hint Rewrite alist_corresponds_to_finite_partial_map_iff : simplication_hints.
